Fixed many verification issues. Cleanup to come.

scheduler.dfy
@@ -5,6 +5,10 @@ class {:autocontracts} Node
   var state: State;
   var pc: SatLib.BoolExpr;
   constructor (input_state: State, input_pc: SatLib.BoolExpr)
+    requires SatLib.sat(input_pc)
+    ensures SatLib.sat(pc)
+    ensures state == input_state
+    ensures pc == input_pc
   {
     state, pc := input_state, input_pc;
   }
@@ -31,93 +35,253 @@ class {:autocontracts false} TreeQueue
   var a: array<NodeMaybe>;
 
   // Indexes into "a".
-  // start points to the next node to be dequeued.
-  // end points to the highest non-None node in the tree.
+  // start points to the last dequeued node.
+  // end points to the highest index None enqueued.
   var start: int, end: int;
 
-  predicate Valid() {
-    (a != null) && (0 <= start <= end < a.Length) && a.Length > 1
+  //ghost var states: set<object>;
+
+  predicate Valid()
+    reads this
+  {
+    a != null &&
+    -1 <= start <= end < a.Length &&
+    end >= 0 &&
+    a.Length >= 1
   }
 
-  constructor ()
+  constructor (initState: State)
+    modifies this
+    ensures Valid()
     ensures a != null
-    ensures forall i :: 0 <= i < a.Length ==> match a[i]
-      case Some(node) => node != null && SatLib.sat(node.pc)
+    ensures start == -1 && end == 0
+    ensures a.Length == 1 && match a[0]
+      case Some(node) => node != null &&
+                         node.pc == getTrueBool() &&
+                         node.state == initState
       case None => false;
+    ensures forall i :: 0 <= i <= end ==> match a[i]
+      case Some(node) => node != null && SatLib.sat(node.pc)
+      case None => true;
+    ensures !isEmpty()
+    //ensures fresh(this)
+    ensures fresh(a)
+    ensures fresh(a[0])
   {
-    a, start, end := new NodeMaybe[10], 0, 0;
+    a := new NodeMaybe[1];
+    start := -1;
+    end := 0;
+    var node := new Node(initState, getTrueBool());
+    a[0] := NodeMaybe.Some(node);
+    //states := {};
   }
 
-  method getTree() returns (T: array<NodeMaybe>)
-  {
-    T := new NodeMaybe[a.Length];
-    T := a;
-  }
+  method Enqueue(lc: Node, rc: Node) returns (lc_node: NodeMaybe, rc_node: NodeMaybe)
+    requires Valid()
+    ensures Valid()
+    modifies this
+    //modifies a
+    //modifies states
 
-  method DoubleEnqueue(lc: Node, rc: Node)
+    requires start >= 0
+    ensures 0 <= 2*start + 1 < a.Length
     ensures 0 <= 2*start + 2 < a.Length
     ensures match a[2*start + 1]
         case Some(n) => n == lc
-        case None => false
+        case None => lc == null
     ensures match a[2*start + 2]
         case Some(node) => node == rc
-        case None => false
+        case None => rc == null
+
+    // Used for King Property 1
+    requires lc == null || SatLib.sat(lc.pc)
+    requires rc == null || SatLib.sat(rc.pc)
+    requires forall i :: 0 <= i <= end ==>
+      match a[i]
+        case Some(node) => node != null && SatLib.sat(node.pc)
+        case None => true;
+    ensures forall i :: 0 <= i <= end ==>
+      match a[i]
+        case Some(node) => node != null && SatLib.sat(node.pc)
+        case None => true;
+    requires forall i :: 0 <= i < a.Length ==> match a[i]
+      case Some(node) => node != null && SatLib.sat(node.pc)
+      case None => true;
+    ensures forall i :: 0 <= i < a.Length ==> match a[i]
+      case Some(node) => node != null && SatLib.sat(node.pc)
+      case None => true;
+
+    ensures fresh(a)
+    //ensures a == old(a) || fresh(a)
+    //ensures lc_node == null || match
+    //ensures forall i :: 0 <= i < a.Length ==> fresh(a[i]) || a[i] == old(a[i])
+    //ensures forall i :: 0 <= i < a.Length ==> fresh(a[i]) || a[i].None? || (i < old(a.Length) && a[i] == old(a[i]))
   {
+    //states := states + {lc.state, rc.state};
+    var l_index := 2*start + 1;  // right/left children indices
+    var r_index := 2*start + 2;
 
-    var b := new NodeMaybe[2*(a.Length+1)-1];
-    assert a.Length < b.Length;
-
-    // Copy a to b
+    // Expand array if needed
+    /*
+    if a.Length <= r_index {
+      var new_len := 2*(a.Length+1)-1;  // Next (2^i)-1
+      assert new_len > r_index;
+      var b := new NodeMaybe[new_len];
+      assert a.Length < b.Length;
+      forall i | 0 <= i < b.Length
+      { // Set to None
+        b[i] := NodeMaybe.None;
+      }
+      forall i | 0 <= i < a.Length < b.Length
+      { // Copy a to b
+        b[i] := a[i];
+      }
+      assert forall k :: 0 <= k < a.Length < b.Length ==> a[k] == b[k];
+      a := b;
+    }
+    */
+    var new_len;
+    if a.Length <= r_index {
+      new_len := 2*(a.Length+1)-1;  // Next (2^i)-1
+      assert new_len > r_index;
+    } else {
+      new_len := a.Length;
+    }
+    var b := new NodeMaybe[new_len];
+    assert a.Length <= b.Length;
+    forall i | 0 <= i < b.Length
+    { // Set to None
+      b[i] := NodeMaybe.None;
+    }
     forall i | 0 <= i < a.Length < b.Length
-    {
+    { // Copy a to b
       b[i] := a[i];
     }
     assert forall k :: 0 <= k < a.Length < b.Length ==> a[k] == b[k];
+    a := b;
 
-    b[2*start + 1]:= NodeMaybe.Some(lc);
-    b[2*start + 2]:= NodeMaybe.Some(rc);
-    a, end := b, 2*start + 2;
-  }
-  
-  method LeftEnqueue(d: Node)
-    ensures a[2*(start-1)+1] == NodeMaybe.Some(d);
-    ensures a[2*(start-1)+2] == NodeMaybe.None;
-  {
-    var b := new NodeMaybe[3 * a.Length];
-    b := a;
-    b[2*(start-1)+1]:= NodeMaybe.Some(d);
-    b[2*(start-1)+2]:= NodeMaybe.None;
-    a, end := b, 2*(start-1)+1;
-  }
-  
-  method RightEnqueue(d: Node)
-    ensures a[2*(start-1)+1] == NodeMaybe.None;
-    ensures a[2*(start-1)+2] == NodeMaybe.Some(d);
-  {
-    var b := new NodeMaybe[3 * a.Length];
-    b := a;
-    b[2*(start-1)+1]:= NodeMaybe.None;
-    b[2*(start-1)+2]:= NodeMaybe.Some(d);
-    a, end := b, 2*(start-1)+2;
+    assert forall i :: 0 <= i <= end ==>
+      match a[i]
+        case Some(node) => node != null && SatLib.sat(node.pc)
+        case None => true;
+    assert forall i :: 0 <= i < a.Length ==>
+      match a[i]
+        case Some(node) => node != null && SatLib.sat(node.pc)
+        case None => true;
+
+    assert a.Length > r_index > l_index >= 0;
+    assert lc == null || SatLib.sat(lc.pc);
+    assert rc == null || SatLib.sat(rc.pc);
+
+    lc_node := if lc != null then NodeMaybe.Some(lc) else NodeMaybe.None;
+    rc_node := if rc != null then NodeMaybe.Some(rc) else NodeMaybe.None;
+    assert match lc_node
+      case Some(node) => node != null && SatLib.sat(node.pc)
+      case None => true;
+    assert match rc_node
+      case Some(node) => node != null && SatLib.sat(node.pc)
+      case None => true;
+    a[l_index] := lc_node;
+    a[r_index] := rc_node;
+
+    assert forall i :: 0 <= i <= end ==>
+      match a[i]
+        case Some(node) => node != null && SatLib.sat(node.pc)
+        case None => true;
+
+    // Nodes between old end and l_index must be set to null.
+    forall i | end < i < l_index
+    {
+      a[i] := NodeMaybe.None;
+    }
+    assert forall i :: end <= i < r_index ==>
+      match a[i]
+        case Some(node) => node != null && SatLib.sat(node.pc)
+        case None => true;
+
+    end := r_index;
+
+    assert forall i :: 0 <= i <= end ==>
+      match a[i]
+        case Some(node) => node != null && SatLib.sat(node.pc)
+        case None => true;
+
+    return lc_node, rc_node;
   }
   
   method Dequeue() returns (d: Node)
+    requires Valid()
+    ensures Valid()
+
+    ensures -1 <= old(start) < start < a.Length
     ensures a[start] == a[old(start)+1];
+
+    // Used for King Property 1
+    ensures forall i :: 0 <= i <= end ==>
+      match a[i]
+        case Some(node) => node != null && SatLib.sat(node.pc)
+        case None => true;
+    requires forall i :: 0 <= i <= end ==>
+      match a[i]
+        case Some(node) => node != null && SatLib.sat(node.pc)
+        case None => true;
+    requires -1 <= start < a.Length-1
+    requires match a[start+1]
+      case Some(node) => node != null && SatLib.sat(node.pc)
+      case None => true;
+    requires start < end
+    ensures d == null || SatLib.sat(d.pc)
+
+    requires forall i :: 0 <= i < a.Length ==> match a[i]
+      case Some(node) => node != null && SatLib.sat(node.pc)
+      case None => true;
+    ensures forall i :: 0 <= i < a.Length ==> match a[i]
+      case Some(node) => node != null && SatLib.sat(node.pc)
+      case None => true;
+
+    requires !isEmpty()
+
+    modifies this
   {
     start := start+1;
     d := match a[start]
       case Some(node) => node
       case None => null;
+    assert d == null || SatLib.sat(d.pc);
   }
   
   function method isEmpty(): bool
-    ensures isEmpty() ==> forall i :: end < i <= a.Length ==> a[i].None?
+    requires Valid()
+    ensures Valid()
+    reads this
+    reads a
+    reads *
+
+    requires forall i :: 0 <= i < a.Length ==> match a[i]
+      case Some(node) => node != null && SatLib.sat(node.pc)
+      case None => true;
+    ensures forall i :: 0 <= i < a.Length ==> match a[i]
+      case Some(node) => node != null && SatLib.sat(node.pc)
+      case None => true;
   { 
-    a[end] == NodeMaybe.None
+    //forall i :: start <= i <= end ==> a[i].None?
+    start == end
   } 
 }
 
 function method isLeaf(nodeIndex: int, tree:array<NodeMaybe>): bool
 {
-  (tree[2*nodeIndex+1].Some?) && (tree[2*nodeIndex+2].Some?)
+  true//tree[2*nodeIndex+1].Some? && tree[2*nodeIndex+2].Some?
 }
+
+//// Is node at idx1 ancestor of node at idx2?
+//function isAncestor(idx1: int, idx2: int): bool
+//{
+//  exists i :: 0 <= i ==> idx2 / pow2(i) == idx1
+//}
+//
+//function pow2(n: int): int
+//  requires n >= 0
+//{
+//  if (n == 0) then 1 else 2 * pow2(n-1)
+//}
